# [Problem link](https://www.codechef.com/problems/P5149)

## PREREQUISITES:
Dynamic programming

## PROBLEM:

For a binary string $S$, define $f(S)$ as follows:
- $\vert S \vert - 1$ times, delete one character from $S$.
- Then, add to the score the number of pairs of adjacent characters that differ.

You’re given $S$, compute the sum of $f(S[i \dots j])$ across all $1 \leq i \leq j \leq N$, i.e., across all substrings of $S$.

## EXPLANATION:

It is recommended to read the editorial of the easy version first.

Recall that the score of a string of length $N$, with $k$ adjacent different characters initially, is 

$$
(N - 1 - k) \cdot k + (0 + 1 + 2 + \dots + k - 1)
$$

The key idea behind solving this version of the problem, is noticing how this value changes when we append a character to $S$.

Suppose $S$ currently ends with a $0$. Then,

- If we append a $0$ to $S$, $N$ increases by 1 but $k$ doesn’t change.
  So, the score increases by exactly $k$.
- If we append a $1$ to $S$, $N$ and $k$ both increase by 1.
  Let $k_0$ denote the old value of $k$, and $k_1$ denote the new one ($k_1 = k_0 + 1$).
  Similarly, let $N_0$ and $N_1$ denote the old and new values of $N$.
  We see that:
  - $N_1 - 1 - k_1 = (N_0 + 1) - 1 - (k_0 + 1) = N_0 - 1 - k_0$.
  - So, $(N_1 - 1 - k_1) \cdot k_1 = (N_0 - 1 - k_0) \cdot (k_0 + 1) = (N_0 - 1 - k_0) \cdot k_0 + (N_0 - 1 - k_0)$.
  - $0 + (1 + \dots + k_1 - 1) = (0 + 1 + \dots + k_0 - 1) + k_0$.
  - So, the overall change in the sum is $(N_0 - 1 - k_0) + k_0 = N_0 - 1$.

tl;dr when we append a new character,

1. If the new character equals the previous last character, the score increases by $k$.
2. Otherwise, the score increases by the initial length minus 1.

---

Let’s define $a_i$ to be the sum of scores of all substrings ending at index $i$.  
We’ll compute $a_i$ from $a_{i-1}$, using the observation above.

There are two cases.

First, suppose $S_i \neq S_{i-1}$.  
Since the last character is different from the previous one, for any substring, the increase in score is its length minus 1.  
We have one substring of every length from 1 to $i-1$, so the overall increase in score across them all is 

$$
0 + 1 + 2 + \dots + i - 2 = \frac{(i-2) \cdot (i-1)}{2}
$$

So, we obtain $a_i = a_{i-1} + \frac{(i-2) \cdot (i-1)}{2}$.

Next, suppose $S_i = S_{i-1}$.  
The last character is the same as the previous one, so the increase in score is the value of $k$.  
So, we need to know the sum of $k$-values of all substrings ending at index $i-1$.  
Let’s store this too, say as the value $b_i$.  
We then obtain $a_i = a_{i-1} + b_{i-1}$.

The array $b$ can be updated by similarly considering two cases:

1. If $S_i \neq S_{i-1}$, the $k$-value of every substring increases by 1.
   So, $b_i = b_{i-1} + i - 1$.
2. Otherwise, the $k$-values of every substring don’t change; so $b_i = b_{i-1}$.

Finally, since $a_i$ represents the sum of scores of all substrings ending at index $i$, the final answer is the sum of the array $a$.

**TIME COMPLEXITY:**

$O(N)$ per testcase.

## CODE
```python
mod = 10**9 + 7
for _ in range(int(input())):
    n = int(input())
    s = input()
    ans = x = sm = 0
    for i in range(1, n):
        if s[i] == s[i-1]:
            x = (x + sm) % mod
        else:
            x = (x + i*(i-1)//2) % mod
            sm = (sm + i) % mod
        ans = (ans + x) % mod
    print(ans)
```
